some tweak

platform/cito/SetModule.v
@@ -4,38 +4,25 @@ Set Implicit Arguments.
 
 Module Type Set_ (Key : MiniDecidableType).
 
-  Delimit Scope set_scope with set.
-
-  Local Open Scope set_scope.
-
   Parameter set : Type.
 
   Parameter mem : Key.t -> set -> Prop.
-  Infix "%in" := mem (at level 60): set_scope.
 
   Parameter union : set -> set -> set.
-  Infix "+" := union : set_scope.
+
+  Parameter union_has_left : forall a b x, mem x a -> mem x (union a b).
+
+  Parameter union_has_right : forall a b x, mem x b -> mem x (union a b).
+
+  Parameter union_elim : forall a b x, mem x (union a b) -> mem x a \/ mem x b.
 
   Parameter empty : set.
-  Notation "{}" := empty : set_scope.
 
-  Parameter singleton : Key.t -> set.
-  Notation "{ x }" := (singleton x) : set_scope.
+  Parameter empty_correct : forall x, ~ mem x empty.
 
-  Parameter singleton_mem : forall x, mem x {x}.
+  Parameter add : set -> Key.t -> set.
 
-  Parameter subset : set -> set -> Prop.
-  Infix "<=" := subset : set_scope.
-
-  Parameter subset_correct : forall a b, a <= b -> forall x, x %in a -> x %in b.
-
-  Parameter subset_refl : forall s, s <= s.
-
-  Parameter subset_union_2 : forall a b, a <= a + b.
-
-  Parameter subset_union_1 : forall a b, a <= b + a.
-
-  Parameter union_same_subset : forall s, s + s <= s.
+  Parameter add_added : forall s x, mem x (add s x).
 
 End Set_.
 
@@ -47,25 +34,17 @@ Module Type MembershipDecidableSet (Key : MiniDecidableType) <: Set_ Key.
 
 End MembershipDecidableSet.
 
-(* Implementations *)
+Module Notations (Key : MiniDecidableType) (Import S : Set_ Key).
+  Delimit Scope set_scope with set.
+  Infix "%in" := mem (at level 60): set_scope.
+  Infix "+" := union : set_scope.
+  Notation "{}" := empty : set_scope.
+End Notations.
 
-Module ArrowSet (Key : MiniDecidableType) : MembershipDecidableSet Key.
-
-  Definition set := Key.t -> bool.
-
-  Definition mem x (s : set) := s x = true.
-
-  Definition union (a b : set) := fun x => orb (a x) (b x).
-
-  Definition empty : set := fun _ => false.
-
-  Definition singleton a : set := fun x => if Key.eq_dec x a then true else false.
-
-  Lemma singleton_mem : forall x, mem x (singleton x).
-    unfold singleton, mem; intros; destruct (Key.eq_dec x x); eauto.
-  Qed.
+Module Relations (Key : MiniDecidableType) (Import S : Set_ Key).
 
   Definition subset (a b : set) := forall x, mem x a -> mem x b.
+  Infix "<=" := subset : set_scope.
 
   Lemma subset_correct : forall a b, subset a b -> forall x, mem x a -> mem x b.
     eauto.
@@ -76,22 +55,79 @@ Module ArrowSet (Key : MiniDecidableType) : MembershipDecidableSet Key.
   Qed.
 
   Definition subset_union_2 : forall a b, subset a (union a b).
-    unfold subset, union, mem; intuition.
+    unfold subset; intros; eapply union_has_left; eauto.
   Qed.
   
   Definition subset_union_1 : forall a b, subset a (union b a).
-    unfold subset, union, mem; intuition.
+    unfold subset; intros; eapply union_has_right; eauto.
   Qed.
 
   Definition union_same_subset : forall s, subset (union s s) s.
-    unfold subset, union, mem; intuition.
+    unfold subset; intros; eapply union_elim in H; destruct H; eauto.
+  Qed.
+
+End Relations.
+
+Module Singleton (Key : MiniDecidableType) (Import S : Set_ Key).
+
+  Definition singleton x := add empty x.
+  Notation "{ x }" := (singleton x) : set_scope.
+
+  Lemma singleton_mem : forall x, mem x (singleton x).
+    unfold singleton; intros; eapply add_added.
+  Qed.
+
+End Singleton.
+
+(* Implementations *)
+
+Module ArrowSet (Key : MiniDecidableType) <: MembershipDecidableSet Key.
+
+  Definition set := Key.t -> bool.
+
+  Definition mem x (s : set) := s x = true.
+
+  Definition union (a b : set) := fun x => orb (a x) (b x).
+
+  Lemma union_has_left : forall a b x, mem x a -> mem x (union a b).
+    unfold mem, union; intuition.
+  Qed.
+
+  Lemma union_has_right : forall a b x, mem x b -> mem x (union a b).
+    unfold mem, union; intuition.
+  Qed.
+
+  Lemma union_elim : forall a b x, mem x (union a b) -> mem x a \/ mem x b.
+    unfold mem, union.
+    intros.
     eapply Bool.orb_true_elim in H.
-    destruct H; eauto.
+    destruct H; intuition.
+  Qed.
+  
+  Definition empty : set := fun _ => false.
+
+  Lemma empty_correct : forall x, ~ mem x empty.
+    unfold empty, mem; eauto.
+  Qed.
+
+  Definition add (s : set) x : set :=
+    fun x' =>
+      if Key.eq_dec x' x then
+        true
+      else
+        s x'.
+
+  Lemma add_added : forall s x, mem x (add s x).
+    unfold add, mem; intros; destruct (Key.eq_dec x x); eauto.
   Qed.
 
   Definition mem_dec : forall x s, {mem x s} + {~ mem x s}.
     unfold mem; intros; destruct (Bool.bool_dec (s x) true); intuition.
   Qed.
+
+  Include Notations Key.
+  Include Relations Key.
+  Include Singleton Key.
 
 End ArrowSet.
 
